theories/L1_MalechaQuoted/test_wcbvEval.v
@@ -5,17 +5,40 @@ Add LoadPath "." as L1.
 Require Import Template.Template.
 Require Import Common.RandyPrelude.
 Require Import L1.L1.  (* whole L1 library is exported by L1.L1 *)
-
 Local Open Scope string_scope.
 Local Open Scope bool.
 Local Open Scope list.
 Set Implicit Arguments.
+
+Definition NN := nat.
+Quote Definition q_NN := NN.
+Print  q_NN.
+Quote Definition q_eNN := Eval cbv in NN.
+Print  q_eNN.
+
+Definition LL := list.
+Quote Definition q_LL := LL.
+Print  q_LL.
+Quote Definition q_eLL := Eval cbv in LL.
+Print  q_eLL.
+
+
+(** non-recursive fixpoint has non-null Defs **)
+Fixpoint tst (b:bool) : bool := true.
+Print tst.
+Quote Recursively Definition p_tst := tst.
+Print p_tst.
 
 (** tool to set up examples for testing **)
 Definition exc_wcbvEval (tmr:nat) (pgm:program): exception Term :=
   match program_Program pgm (ret nil) with
     | Exc str => Exc str
     | Ret pgm => wcbvEval tmr (env pgm) (main pgm)
+  end.
+Definition exc_WcbvEval (pgm:program) (ans:term) : Prop :=
+  match program_Program pgm (ret nil), term_Term ans with
+    | Ret pgm, Ret trm => WcbvEval (env pgm) (main pgm) trm
+    | _, _ => False
   end.
 
 
@@ -44,7 +67,19 @@ induction fs; try reflexivity.
 - simpl. rewrite IHfs. reflexivity.
 Qed.
 
-(** parametric datatypes **)
+(** indexed datatypes **)
+Inductive fin : nat -> Set :=
+| f0: fin 0
+| fS: forall (n:nat) (f:fin n), fin (S n).
+
+Definition fiszero (n:nat) (f:fin n) : bool :=
+  match f with
+    | f0 => true
+    | fS _ => false
+  end.
+Quote Recursively Definition p_fiszero := fiszero.
+Print p_fiszero.
+
 Definition blist := (@list ((fun x:Set => x) bool)).
 Quote Recursively Definition clist := blist.
 Print clist.
@@ -52,7 +87,7 @@ Quote Recursively Definition bcons := (@cons bool).
 Print bcons.
 
 Definition xlist := (@list (list bool)).
-Quote Definition qlist := Eval compute in xlist.
+Quote Definition qlist := Eval cbv in xlist.
 Print qlist.
 Quote Recursively Definition qcons :=
   (@cons (list bool): (list bool) -> xlist -> xlist).
@@ -64,43 +99,169 @@ Print Vector.t.
 
 Definition vplus (n:nat) :
   Vector.t nat n -> Vector.t nat n -> Vector.t nat n :=
-  Eval cbv delta beta in (Vector.map2 plus).
+  Eval cbv in (Vector.map2 plus).
 
 Definition vplus01 :=
   (@vplus 1 (Vector.cons nat 0 0 (Vector.nil nat))
           (Vector.cons nat 1 0 (Vector.nil nat))).
 Quote Recursively Definition p_vplus01 := vplus01.
-Quote Definition q_vplus01 := Eval compute in vplus01.
+Quote Definition q_vplus01 := Eval cbv in vplus01.
 Print p_vplus01.
 Goal (exc_wcbvEval 50 p_vplus01) = term_Term q_vplus01.
 compute. reflexivity.
 Qed.
 
+Definition vec1 := Vector.t Set 1.
+Quote Recursively Definition p_vec1 := vec1.
+Quote Definition q_vec1 := Eval cbv in vec1.
+Goal (exc_wcbvEval 50 p_vec1) = term_Term q_vec1.
+compute. reflexivity.
+Qed.
+
+(***  HERE **********
 Definition v01 : Vector.t nat 2 :=
   (Vector.cons nat 0 1 (Vector.cons nat 1 0 (Vector.nil nat))).
 Definition v23 : Vector.t nat 2 :=
   (Vector.cons nat 2 1 (Vector.cons nat 3 0 (Vector.nil nat))).
 Definition vplus0123 := (@vplus 2 v01 v23).
 Quote Recursively Definition p_vplus0123 := vplus0123.
-Quote Definition q_vplus0123 := Eval compute in vplus0123.
-Goal exc_wcbvEval 40 p_vplus0123 = term_Term q_vplus0123.
+Quote Definition q_vplus0123 := Eval cbv in vplus0123.
+Goal exc_wcbvEval 90 p_vplus0123 = Ret prop.
+unfold p_vplus0123.
+ 
+Goal exc_wcbvEval 90 p_vplus0123 = term_Term q_vplus0123.
 compute. reflexivity.
 Qed.
+***********)
+
+(** match with no branches **)
+Definition Fdemo (f:False) : False := match f with end.
+Print Fdemo.
+Quote Recursively Definition p_Fdemo := Fdemo.
+Print p_Fdemo.
+Axiom FF : False.
+Eval compute in (Fdemo FF).
+
+
+(** match: eval type parts of Defs **)
+Definition bb := bool.
+Definition demo (t:True) : bb := match t with I => true end.
+Print demo.
+Eval cbv in demo.
+Quote Recursively Definition p_demo := demo.
+Print p_demo.
+Quote Definition qcbv_demo := Eval native_compute in demo.
+Print qcbv_demo.
+(*** fails **
+Goal exc_wcbvEval 40 p_demo = term_Term qcbv_demo.
+native_compute. reflexivity.
+Qed.
+***)
+
+Definition bb1 := fun (t:True) => bool.
+Definition demo1 (t:True) : (bb1 t) := match t with I => true end.
+Print demo1.
+Eval cbv in demo1.
+Quote Recursively Definition p_demo1 := demo1.
+Print p_demo1.
+Quote Definition qcbv_demo1 := Eval cbv in demo1.
+Print qcbv_demo1.
+
 
 (** Abishek's example **)
-Axiom feq1 : (fun x:nat => x) = (fun x:nat => x+x-x).
+Definition xx := (fun x:nat => x) = (fun x:nat => x+x-x).
+Print xx.
+Eval cbv in xx.
 
-Definition zero :nat :=
+Axiom feq1 : (fun x:nat => x) = (fun x:nat => x+2).
+Print feq1.
+Eval cbv in feq1.
+Definition zero1 : nat :=
   match feq1 with
     | eq_refl => 0
   end.
-
-Quote Recursively Definition p_zero := zero.
-Quote Definition q_zero := Eval compute in zero.
-Goal exc_wcbvEval 40 p_zero = term_Term q_zero.
+Eval cbv in zero1.
+Quote Definition q_zero1 := Eval cbv in zero1.
+Print q_zero1.
+Quote Recursively Definition p_zero1 := zero1.
+Print p_zero1.
+Goal exc_wcbvEval 40 p_zero1 = term_Term q_zero1.
 compute. reflexivity.
 Qed.
 
+(** fails because Coq cbv is not weak ***
+Axiom feq2 : 0 = 0.
+Print feq2.
+Eval cbv in feq2.
+Definition zero2: nat :=
+  match feq2 with
+    | eq_refl => 0
+  end.
+Print zero2.
+Eval cbv in zero2.
+Quote Definition q_zero2 := Eval cbv in zero2.
+Print Template.Ast.
+Print q_zero2.
+Print IDProp.
+Eval cbv in (term_Term, q_zero2).
+Quote Recursively Definition p_zero2 := zero2.
+Print p_zero2.
+Print IDProp.
+Goal exc_wcbvEval 40 p_zero2 = term_Term q_zero2.
+compute. reflexivity.
+***)
+
+Definition Lb (b:bool) : (b = b) := eq_refl b. 
+Definition testLb := Lb (orb true true).
+Quote Recursively Definition p_testLb := testLb.
+Print p_testLb.
+Eval cbv in testLb.
+Quote Definition q_testLb := Eval cbv in testLb.
+Print q_testLb.
+Goal exc_wcbvEval 40 p_testLb = term_Term q_testLb.
+compute. reflexivity.
+Qed.
+
+Definition trivadd := (1 + 0).
+Quote Definition q_trivadd := Eval cbv in trivadd.
+Print q_trivadd.
+Quote Recursively Definition p_trivadd := trivadd.
+Print p_trivadd.
+Goal exc_wcbvEval 100 p_trivadd = term_Term q_trivadd.
+compute. reflexivity.
+Qed.
+
+Axiom ax : forall x:nat, x = x.
+Definition testAx := ax (1 + 0).
+Print testAx.
+Eval cbv in testAx.
+Quote Definition q_testAx := Eval cbv in testAx.
+Print q_testAx.
+Quote Recursively Definition p_testAx := testAx.
+Print p_testAx.
+
+Eval cbv in (program_Program p_testAx (Ret nil)).
+Definition pgm :=
+  match  (program_Program p_testAx (Ret nil)) with
+    | Ret pgm => env pgm
+    | x => nil
+  end.
+Eval compute in pgm.
+Definition main :=
+  match  (program_Program p_testAx (Ret nil)) with
+    | Ret pgm => main pgm
+    | x => prop
+  end.
+Eval compute in main.
+
+(*** HERE ***)
+Goal exc_wcbvEval 40 p_testAx = term_Term q_testAx.
+compute. reflexivity.
+Qed.
+
+Goal exc_wcbvEval 40 p_testAx = term_Term q_testAx.
+compute. reflexivity.
+Qed.
 
 (** type casting ? **)
 Check (cons: forall (A:Set), A -> list A -> list A).
@@ -168,13 +329,13 @@ Print qconsc.
 Quote Definition AppApp1 := ((@cons nat:nat -> list nat -> list nat) 0).
 Print AppApp1.
 Quote Definition AppApp2 :=
-  Eval compute in ((@cons nat:nat -> list nat -> list nat) 0).
+  Eval cbv in ((@cons nat:nat -> list nat -> list nat) 0).
 Print AppApp2.
 ***)
 
 Definition Nat := nat.
 Definition typedef := ((fun (A:Type) (a:A) => a) Nat 1).
-Quote Definition q_typedef := Eval compute in typedef.
+Quote Definition q_typedef := Eval cbv in typedef.
 Quote Recursively Definition p_typedef := typedef.
 Goal
   (exc_wcbvEval 200 p_typedef) = term_Term q_typedef.
@@ -182,7 +343,7 @@ compute. reflexivity.
 Qed.
 
 Definition II := fun (A:Type) (a:A) => a.
-Quote Definition q_II := Eval compute in II.
+Quote Definition q_II := Eval cbv in II.
 Quote Recursively Definition p_II := II.
 Goal
   (exc_wcbvEval 10 p_II) = term_Term q_II.
@@ -200,11 +361,11 @@ Fixpoint ack (n m:nat) {struct n} : nat :=
                  end
              in ackn m
   end.
-Eval compute in ack 3 5.
+Eval cbv in ack 3 5.
 Definition ack35 := (ack 3 5).
 Quote Recursively Definition p_ack35 := ack35.
-Eval compute in (program_Program p_ack35 (Ret nil)).
-Quote Definition q_ack35 := Eval compute in ack35.
+Eval cbv in (program_Program p_ack35 (Ret nil)).
+Quote Definition q_ack35 := Eval cbv in ack35.
 Goal (exc_wcbvEval 3000 p_ack35) = term_Term q_ack35.
 vm_compute. reflexivity.
 Qed.
@@ -220,14 +381,14 @@ Fixpoint taut (n:nat) : tautArg n -> bool :=
     | 0 => (fun x => x)
     | S n => fun x => taut n (x true) && taut n (x false)
   end.
-Eval compute in taut 0 true.
-Eval compute in taut 1 (fun x => x).
-Eval compute in taut 1 (fun x => x || negb x).
+Eval cbv in taut 0 true.
+Eval cbv in taut 1 (fun x => x).
+Eval cbv in taut 1 (fun x => x || negb x).
 (* Pierce *)
 Definition pierce := taut 2 (fun x y => implb (implb (implb x y) x) x).
 Quote Recursively Definition p_pierce := pierce.
-Eval compute in (program_Program p_pierce (Ret nil)).
-Quote Definition q_pierce := Eval compute in pierce.
+Eval cbv in (program_Program p_pierce (Ret nil)).
+Quote Definition q_pierce := Eval cbv in pierce.
 Goal (exc_wcbvEval 23 p_pierce) = term_Term q_pierce.
  unfold exc_wcbvEval, program_Program, p_pierce.
 compute. reflexivity.
@@ -237,7 +398,7 @@ Definition Scomb := taut 3
          (fun x y z => implb (implb x (implb y z))
                              (implb (implb x y) (implb x z))).
 Quote Recursively Definition p_Scomb := Scomb.
-Quote Definition q_Scomb := Eval compute in Scomb.
+Quote Definition q_Scomb := Eval cbv in Scomb.
 Goal  (exc_wcbvEval 50 p_Scomb) = term_Term q_Scomb.
 vm_compute. reflexivity.
 Qed.
@@ -248,7 +409,7 @@ Fixpoint arity (n:nat) (A:Type) : Type :=
     | 0 => A
     | S n => A -> arity n A
   end.
-Eval compute in arity 2 bool.
+Eval cbv in arity 2 bool.
 Inductive bar : Type :=
 | b0: arity 0 bar
 | b1: arity 1 bar.
@@ -300,8 +461,8 @@ Definition sherwood: forest bool :=
   fcons (node true (fcons (node true (leaf false)) (leaf true)))
         (leaf false).
 Quote Recursively Definition p_sherwood_size := (forest_size sherwood).
-Eval compute in (program_Program p_sherwood_size (Ret nil)).
-Quote Definition q_sherwood_size := Eval compute in (forest_size sherwood).
+Eval cbv in (program_Program p_sherwood_size (Ret nil)).
+Quote Definition q_sherwood_size := Eval cbv in (forest_size sherwood).
 Goal (exc_wcbvEval 40 p_sherwood_size) = term_Term q_sherwood_size.
 reflexivity.
 Qed.
@@ -311,7 +472,7 @@ Definition arden: forest bool :=
         (fcons (node true (fcons (node true (leaf false)) (leaf true)))
                (leaf false)).
 Quote Recursively Definition p_arden_size := (forest_size arden).
-Quote Definition q_arden_size := Eval compute in (forest_size arden).
+Quote Definition q_arden_size := Eval cbv in (forest_size arden).
 Goal (exc_wcbvEval 100 p_arden_size) = term_Term q_arden_size.
 vm_compute; reflexivity.
 Qed.
@@ -329,7 +490,7 @@ Definition Foo : nat -> bool -> wwzz -> wwzz :=
     end.
 Definition Foo0ty := (Foo 0 true (ww uu)).
 Quote Recursively Definition p_Foo0ty := Foo0ty.
-Quote Definition q_Foo0ty := Eval compute in Foo0ty.
+Quote Definition q_Foo0ty := Eval cbv in Foo0ty.
 Goal (exc_wcbvEval 23 p_Foo0ty) = term_Term q_Foo0ty.
 reflexivity.
 Qed.
@@ -346,7 +507,7 @@ Definition hd (A:Set) (ls:lst A) (default:A) : A :=
 Quote Recursively Definition p_hd :=
  (@hd bool (@cns bool true (nl bool)) false).
 Quote Definition q_hd :=
-  Eval compute in (@hd bool (@cns bool true (nl bool)) false).
+  Eval cbv in (@hd bool (@cns bool true (nl bool)) false).
 Goal exc_wcbvEval 100 p_hd = term_Term q_hd.
 reflexivity.
 Qed.
@@ -363,7 +524,7 @@ Definition nehd (A:Set) (ls:nelst A) : A :=
 Quote Recursively Definition p_nehd :=
   (@nehd bool (@necns bool true (@nenl bool false))).
 Quote Definition q_nehd :=
-  Eval compute in (@nehd bool (@necns bool true (@nenl bool false))).
+  Eval cbv in (@nehd bool (@necns bool true (@nenl bool false))).
 Goal exc_wcbvEval 100 p_nehd = term_Term q_nehd.
 reflexivity.
 Qed.
@@ -378,7 +539,7 @@ Definition occIn (A:Set) (t:tm A) : nat :=
     | cc _ => 0
 end.
 Quote Recursively Definition p_occIn := (occIn (cc true)).
-Quote Definition q_occIn := Eval compute in (occIn (cc true)).
+Quote Definition q_occIn := Eval cbv in (occIn (cc true)).
 Goal exc_wcbvEval 20 p_occIn = term_Term q_occIn.
 reflexivity.
 Qed.
@@ -395,13 +556,13 @@ Fixpoint slowFib (n:nat) : nat :=
   end.
 
 Quote Recursively Definition p_slowFib1 := (slowFib 1).
-Quote Definition q_slowFib1 := Eval compute in (slowFib 1).
+Quote Definition q_slowFib1 := Eval cbv in (slowFib 1).
 Goal exc_wcbvEval 10 p_slowFib1 = term_Term q_slowFib1.
 reflexivity.
 Qed.
 
 Quote Recursively Definition p_slowFib3 := (slowFib 3).
-Quote Definition q_slowFib3 := Eval compute in (slowFib 3).
+Quote Definition q_slowFib3 := Eval cbv in (slowFib 3).
 Goal exc_wcbvEval 100 p_slowFib3 = term_Term q_slowFib3.
 compute; reflexivity.
 Qed.
@@ -422,19 +583,19 @@ Qed.
 ***)
 
 Quote Recursively Definition p_fib3 := (fib 3).
-Quote Definition q_fib3 := Eval compute in (fib 3).
+Quote Definition q_fib3 := Eval cbv in (fib 3).
 Goal exc_wcbvEval 100 p_fib3 = term_Term q_fib3.
 vm_compute; reflexivity.
 Qed.
 
 Quote Recursively Definition p_fib5 := (fib 5).
-Quote Definition q_fib5 := Eval compute in (fib 5).
+Quote Definition q_fib5 := Eval cbv in (fib 5).
 Goal exc_wcbvEval 100 p_fib5 = term_Term q_fib5.
 vm_compute; reflexivity.
 Qed.
 
 Quote Recursively Definition p_fib10 := (fib 10).
-Quote Definition q_fib10 := Eval compute in (fib 10).
+Quote Definition q_fib10 := Eval cbv in (fib 10).
 Goal exc_wcbvEval 300 p_fib10 = term_Term q_fib10.
 vm_compute; reflexivity.
 Qed.
@@ -455,13 +616,13 @@ with forest_size1 (f:forest bool) : nat :=
 End S1.
 
 Quote Recursively Definition p_forest_size1 := (forest_size1 1 sherwood).
-Quote Definition q_forest_size1 := Eval compute in (forest_size1 1 sherwood).
+Quote Definition q_forest_size1 := Eval cbv in (forest_size1 1 sherwood).
 Goal (exc_wcbvEval 40 p_forest_size1) = term_Term q_forest_size1.
 vm_compute; reflexivity.
 Qed.
 
 Quote Recursively Definition p_arden_size1 := (forest_size arden).
-Quote Definition q_arden_size1 := Eval compute in (forest_size arden).
+Quote Definition q_arden_size1 := Eval cbv in (forest_size arden).
 Goal (exc_wcbvEval 100 p_arden_size1) = term_Term q_arden_size1.
 vm_compute; reflexivity.
 Qed.
